Refine umax to work with domain in Prop, fixes Pi parametricity

theories/Typing.v
@@ -258,8 +258,10 @@ Definition usup m i :=
   if isProp m then 0 else S i.
 
 (** Maximum of a universe **)
-Definition umax m i j :=
-  if isProp m then 0 else max i j.
+Definition umax mx m i j :=
+  if isProp m then 0
+  else if isProp mx then j
+  else max i j.
 
 Inductive typing (Γ : context) : term → term → Prop :=
 
@@ -278,7 +280,7 @@ Inductive typing (Γ : context) : term → term → Prop :=
       cscoping (Γ ,, (mx, A)) B mKind →
       Γ ⊢ A : Sort mx i →
       Γ ,, (mx, A) ⊢ B : Sort m j →
-      Γ ⊢ Pi i j m mx A B : Sort m (umax m i j)
+      Γ ⊢ Pi i j m mx A B : Sort m (umax mx m i j)
 
 | type_lam :
     ∀ mx m i j A B t,
